Replaced strings with natural numbers in the big example trace to give a factor of 15 speed up.

examples/Sugar2/regexp/regexpLib.sig
@@ -4,4 +4,4 @@
 (* An automata-based matcher added by Joe Hurd                               *)
 (*---------------------------------------------------------------------------*)
 
-signature regexpLib = sig end
+signature regexpLib = sig include regexpTools end
